Define inf_term_path

extracted/sld_interpreter.hs
@@ -108,16 +108,17 @@ eq_dec :: Nat -> Nat -> Sumbool
 eq_dec n =
   nat_rec (\m -> case m of {
                   O -> Left;
-                  S _ -> Right}) (\_ iHn m ->
-    case m of {
-     O -> Right;
-     S n0 -> iHn n0}) n
+                  S _ -> Right})
+    (\_ iHn m -> case m of {
+                  O -> Right;
+                  S n0 -> iHn n0})
+    n
 
 map :: (a1 -> a2) -> (List a1) -> List a2
 map f l =
   case l of {
    Nil -> Nil;
-   Cons a t -> Cons (f a) (map f t)}
+   Cons a l0 -> Cons (f a) (map f l0)}
 
 type Name = Nat
 
@@ -227,7 +228,9 @@ mgu_result_exists t1 t2 =
                  case x1 of {
                   Some s -> ExistT (Some (compose (singleton_subst n t3) s))
                    __;
-                  None -> ExistT None __}}}}) __ x0) (Pair t1 t2)}
+                  None -> ExistT None __}}}})
+           __ x0)
+         (Pair t1 t2)}
   in
   eq_rec_r __ (\h0 -> h0) __ h
 
@@ -312,7 +315,8 @@ eval_step_exists nst =
      Fresh g0 -> ExistT Step (ExistT NoCutting (ExistT (NTState (Leaf 
       (g0 n) s (S n))) __));
      Invoke n0 t -> ExistT Step (ExistT NoCutting (ExistT (NTState (Leaf
-      (proj1_sig (prog n0) t) s n)) __))}) (\c _ iHnst1 nst2 _ ->
+      (proj1_sig (prog n0) t) s n)) __))})
+    (\c _ iHnst1 nst2 _ ->
     case iHnst1 of {
      ExistT x s ->
       case s of {
@@ -337,7 +341,8 @@ eval_step_exists nst =
                StopCutting -> ExistT x (ExistT NoCutting (ExistT (NTState n)
                 __));
                KeepCutting -> ExistT x (ExistT YesCutting (ExistT (NTState n)
-                __))}}}}}}) (\_ iHnst g ->
+                __))}}}}}})
+    (\_ iHnst g ->
     case iHnst of {
      ExistT x s ->
       case s of {
@@ -355,7 +360,8 @@ eval_step_exists nst =
              Step -> ExistT Step (ExistT x0 (ExistT (NTState (Prod0 n g))
               __));
              Answer s1 n0 -> ExistT Step (ExistT x0 (ExistT (NTState (Sum
-              KeepCutting (Leaf g s1 n0) (Prod0 n g))) __))}}}}}) nst
+              KeepCutting (Leaf g s1 n0) (Prod0 n g))) __))}}}}})
+    nst
 
 type Trace = Stream Label
 
